ByteBlockCacheSystem/Marshalling.i.dfy
@@ -287,10 +287,9 @@ module Marshalling {
   ensures s.Some? ==> s.value.graph.Keys == s.value.locs.Keys
   ensures s.Some? ==> forall v | v in s.value.locs.Values :: DiskLayout.ValidNodeLocation(v)
   ensures s.Some? ==> forall ref | ref in s.value.graph :: |s.value.graph[ref]| <= MaxNumChildren()
-  ensures s.Some? ==> forall ref | ref in s.value.graph :: ref <= s.value.refUpperBound
   {
     if |a| == 0 then
-      Some(IndirectionTable(map[], map[], 0))
+      Some(IndirectionTable(map[], map[]))
     else (
       var res := valToIndirectionTableMaps(DropLast(a));
       match res {
@@ -304,8 +303,7 @@ module Marshalling {
           if ref in table.graph || !DiskLayout.ValidNodeLocation(loc) || |succs| as int > MaxNumChildren() then (
             None
           ) else (
-            var upperBound := if ref > table.refUpperBound then ref else table.refUpperBound;
-            Some(IndirectionTable(table.locs[ref := loc], table.graph[ref := succs], upperBound)) // yizhou7: TODO
+            Some(IndirectionTable(table.locs[ref := loc], table.graph[ref := succs]))
           )
         )
         case None => None
